Improved coqdoc. Some cleanup.

theories/Misc.v
@@ -1,7 +1,14 @@
+(** * Some facts not found in the standard library *)
+
 From ConCert Require Import CustomTactics.
 From MetaCoq Require Import utils.
 Require Import List.
 
+Import ListNotations.
+Import Lia.
+
+Definition fun_prod {A B C D} (f : A -> C) (g : B -> D) : A * B -> C * D :=
+  fun x => (f (fst x), g (snd x)).
 
 Lemma forallb_Forall_iff {A} (p : A -> bool) (l : list A):
   Forall (fun x => p x = true) l <-> forallb p l = true.
@@ -43,3 +50,98 @@ Proof.
   induction l;simpl;intros p q Hfa H;auto.
   inv_andb Hfa. split_andb;try eapply IHl;eauto.
 Qed.
+
+Lemma Forall_In {A} x (xs : list A) P :
+  In x xs ->
+  Forall P xs ->
+  P x.
+Proof.
+  revert x.
+  induction xs;intros x Hin Hfa;auto.
+  * inversion Hin.
+  * simpl in *. destruct Hin;subst; inversion Hfa;eauto.
+Qed.
+
+Lemma forallb_In {A} x (xs : list A) p :
+  In x xs ->
+  forallb p xs ->
+  p x.
+Proof.
+  revert x.
+  induction xs;intros x Hin Hfa;auto.
+  simpl in *. inv_andb Hfa;intuition;subst;auto.
+Qed.
+
+
+Definition from_option {A : Type} ( o : option A) (default : A) :=
+  match o with
+  | None => default
+  | Some v => v
+  end.
+
+
+Lemma from_option_indep {A} (o : option A) d  d' v :
+  o = Some v -> from_option o d = from_option o d'.
+Proof.
+  intros;subst;easy.
+Qed.
+
+Section CombineProp.
+
+  Lemma combine_app : forall A B (l2 l2': list B) (l1 l1' : list A),
+    #|l1| = #|l2| ->
+    combine (l1 ++ l1') (l2 ++ l2') = combine l1 l2 ++ combine l1' l2'.
+  Proof.
+    induction l2.
+    + simpl. intros l2' l1 l1' Heq. destruct l1;tryfalse;reflexivity.
+    + simpl. intros l2' l1 l1' Heq. destruct l1;cbn; inversion Heq.
+      simpl. apply f_equal2;eauto.
+  Qed.
+
+  Lemma combine_rev : forall A B (l2 : list B) (l1 : list A),
+    #|l1| = #|l2| ->
+    combine (rev l1) (rev l2) = rev (combine l1 l2).
+  Proof.
+    intros A B.
+    induction l2 using utils.rev_ind.
+    + simpl. intros l1 Heq. destruct l1;eauto.
+      simpl;destruct (rev l1 ++ [a]);reflexivity.
+    + simpl. intros l1 Heq. destruct l1 using utils.rev_ind;auto.
+      repeat rewrite app_length in Heq;simpl in *.
+      assert (#|l1| = #|l2|) by lia.
+      repeat rewrite rev_unit. simpl.
+      rewrite IHl2 by auto.
+      rewrite combine_app by auto.
+      simpl. now rewrite rev_unit.
+  Qed.
+
+  Lemma map_combine_snd : forall A B (l2 : list B) (l1 : list A),
+    #|l1| = #|l2| ->
+   map snd (combine l1 l2) = l2.
+  Proof.
+    induction l2.
+    + simpl. intros l1 Heq. destruct l1;reflexivity.
+    + simpl. intros l1 Heq. destruct l1;cbn. inversion Heq.
+      simpl. apply f_equal2;eauto.
+  Qed.
+
+
+  Lemma map_map_combine_snd : forall A B C (f : B -> C) (l2 : list B) (l1 : list A),
+      #|l1| = #|l2| ->
+      (map f l2) = map f (map snd (combine l1 l2)).
+  Proof.
+    intros; now rewrite map_combine_snd.
+  Qed.
+
+  Lemma map_combine_snd_funprod :
+    forall A B C (f : B -> C) (l1 : list A) (l2 : list B),
+      map (fun_prod id f) (combine l1 l2) = combine l1 (map f l2).
+  Proof.
+    induction l1;intros.
+    + reflexivity.
+    + destruct l2.
+      * reflexivity.
+      * cbn. f_equal. apply IHl1.
+  Qed.
+
+End CombineProp.
