theories/Wf.v
@@ -1,0 +1,118 @@
+(** * Well-formedness conditions  *)
+
+Require Import List Bool Relations Morphisms ssrbool.
+Require Import MetaCoq.Template.utils.
+
+Require Import Ast EnvSubst.
+Require Import EvalE.
+Require Import MyEnv.
+
+Import NamelessSubst.
+
+Definition is_type e : bool :=
+  match expr_to_ty e with
+  | Some _ => true
+  | _ => false
+  end.
+
+(** Well-formed constructor in the definition of an inductive *)
+Definition constr_ok (nparam : nat) (c : constr) : bool :=
+  forallb (iclosed_ty nparam) (map snd c.2).
+
+(** Well-formed global geclarations *)
+Definition global_dec_ok (gd : global_dec) : bool :=
+  match gd with
+  | gdInd _ nparam cs _ => forallb (constr_ok nparam) cs
+  end.
+
+(** Well-formed global environment *)
+Definition genv_ok Σ := forallb global_dec_ok Σ.
+
+
+(** Well-formedness condition in evaluation environments wrt. a type: [ρ] is well-formed wrt. a type [ty] when for any type variables mentioned in [ty], if there is a corresponding expression in ρ (starting from the index [n]) it corresponds to a type. *)
+  Fixpoint ty_env_ok (n : nat) (ρ : env expr) (ty : type): bool :=
+    match ty with
+    | tyInd x => true
+    | tyForall v ty0 => ty_env_ok (S n) ρ ty0
+    | tyApp ty1 ty2 => ty_env_ok n ρ ty1 && ty_env_ok n ρ ty2
+    | tyVar _ => false
+    | tyRel i => if Nat.leb n i then
+                  match lookup_i ρ (i-n) with
+                  | Some e => is_type e (* if there is somethig in [ρ], it must be a type *)
+                  | None => true (* if nothing there, that's ok *)
+                  end
+                else true
+    | tyArr ty1 ty2 => ty_env_ok n ρ ty1 && ty_env_ok n ρ ty2
+    end.
+
+  (** Well-formedness condition in evaluation environments wrt. an expression ((WF.i) in the paper): [ρ] is well-formed wrt. an expression [e] when for any type variables mentioned in [e], if there is a corresponding expression in ρ (starting from the index [n]) it corresponds to a type. *)
+  Definition ty_expr_env_ok (ρ : env expr) : nat -> expr -> bool:=
+    fix rec n e :=
+      match e with
+      | eRel i => true
+      | eVar nm  => false
+      | eLambda nm ty b => ty_env_ok n ρ ty && rec (1+n) b
+      | eTyLam nm b => rec (1+n) b
+      | eLetIn nm e1 ty e2 => rec n e1 && ty_env_ok n ρ ty && rec (1+n) e2
+      | eApp e1 e2 => rec n e1 && rec n e2
+      | eConstr t i as e' => true
+      | eConst nm => true
+      | eCase nm_i ty e bs =>
+        let bs'' := List.forallb
+                      (fun x => rec (length (pVars (fst x)) + n) (snd x)) bs in
+        forallb (ty_env_ok n ρ) (snd nm_i) && ty_env_ok n ρ ty && rec n e && bs''
+      | eFix nm v ty1 ty2 b => ty_env_ok n ρ ty1 && ty_env_ok n ρ ty2 && rec (2+n) b
+      | eTy ty => ty_env_ok n ρ ty
+      end.
+
+  (** This predicate defines a subset of types which are values *)
+  Inductive ty_val : type -> Type :=
+  | vtyInd : forall ind, ty_val (tyInd ind)
+  | vtyRel : forall i, ty_val (tyRel i)
+  | vtyForall : forall nm ty , ty_val ty -> ty_val (tyForall nm ty)
+  | vtyApp : forall ty1 ty2 ind tys,
+      decompose_inductive ty1 = Some (ind, tys) ->
+      ty_val ty1 ->
+      ty_val ty2 ->
+      ty_val (tyApp ty1 ty2)
+  | vtyArr : forall ty1 ty2,
+      ty_val ty1 ->
+      ty_val ty2 ->
+      ty_val (tyArr ty1 ty2).
+
+ (** Well-formed value ((WF.iii) in the paper) *)
+ Inductive val_ok Σ : val -> Type :=
+  | vokClosLam : forall e nm ρ ty1 ty2,
+      AllEnv (val_ok Σ) ρ ->
+      ty_expr_env_ok (exprs ρ) 1 e ->
+      iclosed_n (1 + length ρ) e ->
+      iclosed_ty 0 ty1 ->
+      iclosed_ty 0 ty2 ->
+      ty_val ty1 ->
+      ty_val ty2 ->
+      val_ok Σ (vClos ρ nm cmLam ty1 ty2 e)
+  | vokClosFix : forall e nm fixename ρ ty1 ty2,
+      AllEnv (val_ok Σ) ρ ->
+      ty_expr_env_ok (exprs ρ) 2 e ->
+      iclosed_n (2 + length ρ) e ->
+      iclosed_ty 0 ty1 ->
+      iclosed_ty 0 ty2 ->
+      ty_val ty1 ->
+      ty_val ty2 ->
+      val_ok Σ (vClos ρ nm (cmFix fixename) ty1 ty2 e)
+  | vokTyClos : forall e nm ρ,
+      AllEnv (val_ok Σ) ρ ->
+      ty_expr_env_ok (exprs ρ) 1 e ->
+      iclosed_n (1 + length ρ) e ->
+      val_ok Σ (vTyClos ρ nm e)
+  | vokContr : forall i nm vs ci,
+      All (val_ok Σ) vs ->
+      resolve_constr Σ i nm = Some ci ->
+      val_ok Σ (vConstr i nm vs)
+  | vokTy : forall ty,
+      iclosed_ty 0 ty ->
+      ty_val ty ->
+      val_ok Σ (vTy ty).
+
+ (** Well-formed evaluation environment contains well-formed values *)
+ Definition env_ok Σ (ρ : env val) := AllEnv (val_ok Σ) ρ.
